LeanMqtt/Packets/VarHeader/Basic.lean
@@ -12,68 +12,69 @@ open Mqtt
   Determines the Variable Header type based on the Packet Kind
   and the specific flags (needed for Publish QoS).
 -/
-def VarHeader.getType (w : WhichPkt) (f : WhichPkt.flagType w) : Type :=
-  match w with
-  | .connect     => Var_Connect
-  | .connack     => Var_Connack
-  | .publish     => Var_Publish f.qos
-  | .puback      => Var_Puback
-  | .pubrec      => Var_Pubrec
-  | .pubrel      => Var_Pubrel
-  | .pubcomp     => Var_Pubcomp
-  | .subscribe   => Var_Subscribe
-  | .suback      => Var_Suback
-  | .unsubscribe => Var_Unsubscribe
-  | .unsuback    => Var_Unsuback
-  | .pingreq     => Var_Pingreq
-  | .pingresp    => Var_Pingresp
-  | .disconnect  => Var_Disconnect
-  | .auth        => Var_Auth
+def VarHeader.getType (k : PktKind) (f : PktFlags k) : Type :=
+  match k, f with
+  | .connect, _     => Var_Connect
+  | .connack, _     => Var_Connack
+  | .publish, f     => Var_Publish f.qos
+  | .puback, _      => Var_Puback
+  | .pubrec, _      => Var_Pubrec
+  | .pubrel, _      => Var_Pubrel
+  | .pubcomp, _     => Var_Pubcomp
+  | .subscribe, _   => Var_Subscribe
+  | .suback, _      => Var_Suback
+  | .unsubscribe, _ => Var_Unsubscribe
+  | .unsuback, _    => Var_Unsuback
+  | .pingreq, _     => Var_Pingreq
+  | .pingresp, _    => Var_Pingresp
+  | .disconnect, _  => Var_Disconnect
+  | .auth, _        => Var_Auth
 
-def VarHeader.serializeValue {w : WhichPkt} {f : WhichPkt.flagType w}
-  (v : VarHeader.getType w f) : List UInt8 :=
-  match w with
-  | .connect     => Var_Connect.serialize v
-  | .connack     => Var_Connack.serialize v
-  | .publish     => @Var_Publish.serialize f.qos v
-  | .puback      => Var_Puback.serialize v
-  | .pubrec      => Var_Pubrec.serialize v
-  | .pubrel      => Var_Pubrel.serialize v
-  | .pubcomp     => Var_Pubcomp.serialize v
-  | .subscribe   => Var_Subscribe.serialize v
-  | .suback      => Var_Suback.serialize v
-  | .unsubscribe => Var_Unsubscribe.serialize v
-  | .unsuback    => Var_Unsuback.serialize v
-  | .pingreq     => Var_Pingreq.serialize v
-  | .pingresp    => Var_Pingresp.serialize v
-  | .disconnect  => Var_Disconnect.serialize v
-  | .auth        => Var_Auth.serialize v
+def VarHeader.serializeValue {k : PktKind} {f : PktFlags k}
+  (v : VarHeader.getType k f) : List UInt8 :=
+  match k, f with
+  | .connect, _     => Var_Connect.serialize v
+  | .connack, _     => Var_Connack.serialize v
+  | .publish, f     => @Var_Publish.serialize f.qos v
+  | .puback, _      => Var_Puback.serialize v
+  | .pubrec, _      => Var_Pubrec.serialize v
+  | .pubrel, _      => Var_Pubrel.serialize v
+  | .pubcomp, _     => Var_Pubcomp.serialize v
+  | .subscribe, _   => Var_Subscribe.serialize v
+  | .suback, _      => Var_Suback.serialize v
+  | .unsubscribe, _ => Var_Unsubscribe.serialize v
+  | .unsuback, _    => Var_Unsuback.serialize v
+  | .pingreq, _     => Var_Pingreq.serialize v
+  | .pingresp, _    => Var_Pingresp.serialize v
+  | .disconnect, _  => Var_Disconnect.serialize v
+  | .auth, _        => Var_Auth.serialize v
 
-def VarHeader.parserValue (w : WhichPkt) (f : WhichPkt.flagType w) : Parser (VarHeader.getType w f) :=
-  match w with
-  | .connect     => Var_Connect.parser
-  | .connack     => Var_Connack.parser
-  | .publish     => Var_Publish.parser f.qos
-  | .puback      => Var_Puback.parser
-  | .pubrec      => Var_Pubrec.parser
-  | .pubrel      => Var_Pubrel.parser
-  | .pubcomp     => Var_Pubcomp.parser
-  | .subscribe   => Var_Subscribe.parser
-  | .suback      => Var_Suback.parser
-  | .unsubscribe => Var_Unsubscribe.parser
-  | .unsuback    => Var_Unsuback.parser
-  | .pingreq     => Var_Pingreq.parser
-  | .pingresp    => Var_Pingresp.parser
-  | .disconnect  => Var_Disconnect.parser
-  | .auth        => Var_Auth.parser
+def VarHeader.parserValue
+  (k : PktKind) (f : PktFlags k) : Parser (VarHeader.getType k f) :=
+  match k, f with
+  | .connect, _     => Var_Connect.parser
+  | .connack, _     => Var_Connack.parser
+  | .publish, f     => Var_Publish.parser f.qos
+  | .puback, _      => Var_Puback.parser
+  | .pubrec, _      => Var_Pubrec.parser
+  | .pubrel, _      => Var_Pubrel.parser
+  | .pubcomp, _     => Var_Pubcomp.parser
+  | .subscribe, _   => Var_Subscribe.parser
+  | .suback, _      => Var_Suback.parser
+  | .unsubscribe, _ => Var_Unsubscribe.parser
+  | .unsuback, _    => Var_Unsuback.parser
+  | .pingreq, _     => Var_Pingreq.parser
+  | .pingresp, _    => Var_Pingresp.parser
+  | .disconnect, _  => Var_Disconnect.parser
+  | .auth, _        => Var_Auth.parser
 
 abbrev VarHeader (h : FixedHeader) : Type :=
-  VarHeader.getType h.which h.flags
+  VarHeader.getType h.kind h.flags
 
 def VarHeader.serialize (h : FixedHeader) (v : VarHeader h) : List UInt8 :=
   VarHeader.serializeValue v
 
 def VarHeader.parser (h : FixedHeader) : Parser (VarHeader h) :=
-  VarHeader.parserValue h.which h.flags
+  VarHeader.parserValue h.kind h.flags
 
 end Mqtt
